RocqOfRust/revm/revm_interpreter/instructions/simulate/utility.v
@@ -4,6 +4,34 @@ Require Import alloy_primitives.bits.simulate.address.
 Require Import alloy_primitives.bits.simulate.fixed.
 Require Import alloy_primitives.links.aliases.
 Require Import revm.revm_interpreter.instructions.links.utility.
+Require Import ruint.links.lib.
+
+Definition cast_slice_to_u256 (slice : list u8) : aliases.U256.t :=
+  {|
+    Uint.value := List.fold_left (fun acc byte => (acc * 256) + i[byte])%Z slice 0;
+  |}.
+
+Lemma cast_slice_to_address_like
+    (stack : Stack.t)
+    (slice : '& (list u8))
+    (dest : '&mut aliases.U256.t) :
+  SimulateM.eval_f
+    (run_cast_slice_to_u256 slice dest)
+    stack =
+  let*s slice := SimulateM.read stack slice.(Ref.core) in
+  match slice with
+  | Output.Success slice =>
+    let*s stack' := SimulateM.write stack dest.(Ref.core) (cast_slice_to_u256 slice) in
+    match stack' with
+    | Output.Success stack' =>
+      SimulateM.Pure (Output.Success tt, stack')
+    | Output.Exception exception =>
+      SimulateM.Pure (Output.Exception exception, stack)
+    end
+  | Output.Exception exception =>
+    SimulateM.Pure (Output.Exception exception, stack)
+  end.
+Admitted.
 
 Module Impl_IntoAddress_for_U256.
   Definition into_address (self : aliases.U256.t) : Address.t :=
